Update montgomery_ladder.v

montgomery_ladder.v
@@ -1,7 +1,10 @@
 Require Import ZArith.
 Require Import Lia.
+Require Import Coq.Vectors.Vector.
+Require Import Coq.Vectors.Fin.
 From stdpp Require Import base.
 From stdpp Require Import bitvector.
+From stdpp Require Import list.
 
 Open Scope Z_scope.
 
@@ -128,6 +131,11 @@ Section Montgomery.
   Lemma doubling_num_algebra (X Zc : Z) :
     fmul (fsq (fadd X Zc)) (fsq (fsub X Zc)) =
       fsq (fsub (fsq X) (fsq Zc)).
+  Proof.
+    unfold fsq, fadd, fsub, fmul.
+    rewrite ?Zmult_mod_idemp_l, ?Zmult_mod_idemp_r,
+            ?Zminus_mod_idemp_l, ?Zminus_mod_idemp_r.
+    f_equal.
   Admitted.
 
   (* (UT+VW)² = 4(X₂X₃ - Z₂Z₃)²
@@ -360,19 +368,11 @@ Section HammingWeight.
   (* check if mod at every operation? *)
   (* signed or unsigned? *)
 
-  (* Definition fadd (a b : Z) : Z := (a + b) mod p.
-  Definition fsub (a b : Z) : Z := (a - b) mod p.
-  Definition fmul (a b : Z) : Z := (a * b) mod p.
-  Definition fsq  (a : Z)   : Z := fmul a a. *)
-
   (* bv version *)
   Definition fadd_bv (a b : bv n) : bv n := bv_modu (bv_add a b) p .
   Definition fsub_bv (a b : bv n) : bv n := bv_modu (bv_sub a b) p.
   Definition fmul_bv (a b : bv n) : bv n := bv_modu (bv_mul a b) p.
   Definition fsq_bv  (a : bv n)   : bv n := fmul_bv a a.
-
-  Definition num_true (bools : list bool) : nat.
-  Admitted.
 
   Inductive ProbType :=
     | Prob_concrete
@@ -405,12 +405,24 @@ Section HammingWeight.
     | Prob_random, Prob_random => Prob_unknown
     end.
   
-  Definition fadd_probvar (a b : ProbVar) : ProbVar := {| 
+  Definition fadd_probvar (a b : ProbVar) : ProbVar := {|
     Value := fadd_bv a.(Value) b.(Value);
     Ptype := faddsub_prob a.(Ptype) b.(Ptype)
   |}.
 
+  (* NEW: sub and mul *)
+  Definition fsub_probvar (a b : ProbVar) : ProbVar := {|
+    Value := fsub_bv a.(Value) b.(Value);
+    Ptype := faddsub_prob a.(Ptype) b.(Ptype)
+  |}.
+
+  Definition fmul_probvar (a b : ProbVar) : ProbVar := {|
+    Value := fmul_bv a.(Value) b.(Value);
+    Ptype := fmul_prob a.(Ptype) b.(Ptype)
+  |}.
+
   (* another direction: duplicate circuit --> invert? --> HW same without masking *)
+    (* would be cool *)
 
   Inductive ProbHW :=
     | ProbHW_concrete (n : N)
@@ -420,27 +432,643 @@ Section HammingWeight.
   (* Todo: toy example of masking? *)
 
   (* language *)
-  Inductive exp : Type :=
-    | Constant (c : ProbVar)
-    | Add (a b : exp)
-    | Sub (a b : exp)
-    | Mul (a b : exp).
+  Definition var := nat.
+
+  Inductive instr : Type :=
+    (* | Constant (c : ProbVar)
+    | Var      (i : nat) 
+    | Add (a b : var)
+    | Sub (a b : var)
+    | Mul (a b : var). *)
+
+    | IAdd (rd rs1 rs2 : var)
+    | ISub (rd rs1 rs2 : var)
+    | IMul (rd rs1 rs2 : var)
+    | Observe (rd : var).
   
-  Fixpoint interp_exp (e : exp) : ProbVar.
-    refine (match e with
-            | Constant c => c
-            | Add a b => fadd_probvar (interp_exp a) (interp_exp b)
-            (* TODO *)
-            | _ => _
-            end).
+  Open Scope nat.
+
+  Notation rX1  := 0  (only parsing).
+  Notation rX2  := 1  (only parsing).
+  Notation rZ2  := 2  (only parsing).
+  Notation rX3  := 3  (only parsing).
+  Notation rZ3  := 4  (only parsing).
+  Notation rA24 := 5  (only parsing).
+  Notation rU   := 6  (only parsing).   (* X2 + Z2 *)
+  Notation rV   := 7  (only parsing).   (* X2 - Z2 *)
+  Notation rW   := 8  (only parsing).   (* X3 + Z3 *)
+  Notation rT   := 9  (only parsing).   (* X3 - Z3 *)
+  Notation rU2  := 10 (only parsing).   (* U*U *)
+  Notation rV2  := 11 (only parsing).   (* V*V *)
+  Notation rUT  := 12 (only parsing).   (* U*T *)
+  Notation rVW  := 13 (only parsing).   (* V*W *)
+  Notation rSp  := 14 (only parsing).   (* UT + VW *)
+  Notation rSm  := 15 (only parsing).   (* UT - VW *)
+  Notation rX3' := 16 (only parsing).   (* Sp^2 *)
+  Notation rSm2 := 17 (only parsing).   (* Sm^2 *)
+  Notation rZ3' := 18 (only parsing).   (* Sm2 * X1 *)
+  Notation rX2' := 19 (only parsing).   (* U2 * V2 *)
+  Notation rD   := 20 (only parsing).   (* U2 - V2 *)
+  Notation rAD  := 21 (only parsing).   (* A24 * D *)
+  Notation rT2  := 22 (only parsing).   (* V2 + AD *)
+  Notation rZ2' := 23 (only parsing).   (* D * T2 *)
+
+
+  Definition program : list instr :=
+    [ IAdd rU   rX2  rZ2    (* U   = X2 + Z2 *)
+    ; ISub rV   rX2  rZ2    (* V   = X2 - Z2 *)
+    ; IAdd rW   rX3  rZ3    (* W   = X3 + Z3 *)
+    ; ISub rT   rX3  rZ3    (* T   = X3 - Z3 *)
+    ; IMul rU2  rU   rU     (* U2  = U  * U *)
+    ; IMul rV2  rV   rV     (* V2  = V  * V *)
+    ; IMul rUT  rU   rT     (* UT  = U  * T *)
+    ; IMul rVW  rV   rW     (* VW  = V  * W *)
+    ; IAdd rSp  rUT  rVW    (* Sp  = UT + VW *)
+    ; ISub rSm  rUT  rVW    (* Sm  = UT - VW *)
+    ; IMul rX3' rSp  rSp    (* X3' = Sp^2 *)
+    ; IMul rSm2 rSm  rSm    (* Sm2 = Sm^2 *)
+    ; IMul rZ3' rSm2 rX1    (* Z3' = Sm2 * X1 *)
+    ; IMul rX2' rU2  rV2    (* X2' = U2 * V2 *)
+    ; ISub rD   rU2  rV2    (* D   = U2 - V2 *)
+    ; IMul rAD  rA24 rD     (* AD  = A24 * D *)
+    ; IAdd rT2  rV2  rAD    (* T2  = V2 + AD *)
+    ; IMul rZ2' rD   rT2    (* Z2' = D * T2 *)
+    ].
   
-  (* add variables? --> try to implement mont ladder using this language *)
+  (* todo: reuse registers --> use less regs *)
+    (* program counter & fetch memory *)
+
+  Definition ProbEnv := list ProbVar.
+
+  Definition prob_default_var : ProbVar := {|
+    Value := bv_0 n;
+    Ptype := Prob_unknown
+  |}.
+  
+  (* secret register & public register --> only do dual circuits on the secret *)
+
+  Definition prob_read_register (env : ProbEnv) (i : var) : ProbVar := nth i env prob_default_var.
+  Definition prob_write_register (env : ProbEnv) (i : var) (data : ProbVar) : ProbEnv := list_insert i data env.
+
+  Definition num_true (bools : list bool) : nat :=
+    fold_left (fun (acc : nat) (b : bool) => if b then acc + 1 else acc) bools 0.
 
   Definition HW (a : bv n) : nat := num_true (bv_to_bits a).
+
+  Definition num_1s (a : bv n) : nat :=
+    num_true (bv_to_bits a).
   
+  Definition num_1s_in_list (bvs : list (bv n)) : nat :=
+    fold_left (fun acc pv => acc + HW pv) bvs 0.
+
+  Definition num_1s_in_env (env : ProbEnv) : nat :=
+    num_1s_in_list (map Value env).
+
+  Inductive Observation :=
+    | RegObservation (r : var) (val : (bv n)).
+
+  Definition prob_interp_instr (env : ProbEnv) (e : instr) : ProbEnv * list Observation :=
+    match e with
+    (* | Constant c => c *)
+    (* | Var i      => nth i env default_var *)
+    | IAdd rd a b    => (prob_write_register env rd (fadd_probvar (prob_read_register env a) (prob_read_register env b)), [])
+    | ISub rd a b    => (prob_write_register env rd (fsub_probvar (prob_read_register env a) (prob_read_register env b)), [])
+    | IMul rd a b    => (prob_write_register env rd (fmul_probvar (prob_read_register env a) (prob_read_register env b)), [])
+    | Observe rd     => (env, [RegObservation rd (prob_read_register env rd).(Value)])
+    end.
+  
+  Section DualCircuit.
+
+    (* Types & operational semantics *)
+
+    Definition Env := list (bv n).
+    Record state := { env : Env; denv : Env }.
+
+    Definition default_var : bv n := bv_0 n.
+    Definition read_register  (env : Env) (i : var) : bv n      := nth i env default_var.
+    Definition write_register (env : Env) (i : var) (data : bv n) : Env := list_insert i data env.
+
+    Definition interp_instr (env : Env) (e : instr) : Env * list Observation :=
+      match e with
+      | IAdd rd a b => (write_register env rd (fadd_bv (read_register env a) (read_register env b)), [])
+      | ISub rd a b => (write_register env rd (fsub_bv (read_register env a) (read_register env b)), [])
+      | IMul rd a b => (write_register env rd (fmul_bv (read_register env a) (read_register env b)), [])
+      | Observe rd  => (env, [RegObservation rd (read_register env rd)])
+      end.
+
+    (* dual circuit: env holds actual values, denv = map bv_not env *)
+    Definition dual_interp_instr (s : state) (e : instr) : state * list Observation :=
+      let '(env', obs) := interp_instr s.(env) e in
+      ({| env := env'; denv := map bv_not env' |}, obs).
+
+    (* run first [steps] instructions, accumulating observations *)
+    Definition run (s : state) (prog : list instr) (steps : nat) : state * list Observation :=
+      fold_left
+        (fun '(s_acc, obs_acc) e =>
+          let '(s', new_obs) := dual_interp_instr s_acc e in
+          (s', obs_acc ++ new_obs))
+        (firstn steps prog) (s, []).
+
+      
+
+    (* Security definitions *)
+
+    (* invariant: denv is always the bitwise complement of env *)
+    Definition valid_state (s : state) : Prop :=
+      s.(denv) = map bv_not s.(env).
+
+    Definition is_complement (e1 e2 : Env) : Prop :=
+      forall i, read_register e2 i = bv_not (read_register e1 i).
+
+    Definition num_1s_in_state (s : state) : nat :=
+      num_1s_in_list s.(env) + num_1s_in_list s.(denv).
+
+    (* security: total HW per cycle is constant regardless of secret *)
+    Definition secure (prog : list instr) (s : state) :=
+      exists c, forall steps, num_1s_in_state (run s prog steps).1 = c.
+
+
+
+    (* Length preservation *)
+
+    Lemma write_register_length : forall (e : Env) (i : var) (v : bv n),
+      length (write_register e i v) = length e.
+    Proof. intros e i v. unfold write_register. apply length_insert. Qed.
+
+    Lemma interp_instr_preserves_length : forall (e : Env) (i : instr),
+      length (interp_instr e i).1 = length e.
+    Proof.
+      intros e i. destruct i; simpl; rewrite ?write_register_length; reflexivity.
+    Qed.
+
+    Lemma dual_interp_preserves_length : forall (s : state) (i : instr),
+      length (env (dual_interp_instr s i).1) = length (env s).
+    Proof.
+      intros s i. unfold dual_interp_instr.
+      destruct (interp_instr s.(env) i) as [env' obs] eqn:H.
+      simpl. rewrite <- (interp_instr_preserves_length s.(env) i). rewrite H. reflexivity.
+    Qed.
+
+    Lemma fold_left_preserves_length : forall instrs s_init obs_init,
+      length (env (fold_left
+        (fun '(s_acc, obs_acc) e =>
+          let '(s', new_obs) := dual_interp_instr s_acc e in
+          (s', obs_acc ++ new_obs))
+        instrs (s_init, obs_init)).1) = length (env s_init).
+    Proof.
+      induction instrs as [| i rest IH]; intros s_init obs_init.
+      - simpl. reflexivity.
+      - simpl. destruct (dual_interp_instr s_init i) as [s' new_obs] eqn:Hstep.
+        rewrite IH. rewrite <- (dual_interp_preserves_length s_init i).
+        rewrite Hstep. reflexivity.
+    Qed.
+
+    Lemma run_preserves_length : forall (s : state) (prog : list instr) (steps : nat),
+      length (env (run s prog steps).1) = length (env s).
+    Proof. intros s prog steps. unfold run. apply fold_left_preserves_length. Qed.
+
+    
+    
+    (* Valid state preservation *)
+
+    Lemma dual_interp_preserves_valid : forall (s : state) (e : instr),
+      valid_state (dual_interp_instr s e).1.
+    Proof.
+      intros s e. unfold dual_interp_instr, valid_state.
+      destruct (interp_instr s.(env) e) as [env' obs]. simpl. reflexivity.
+    Qed.
+
+    Lemma fold_left_run_valid : forall instrs s_init obs_init,
+      valid_state s_init ->
+      valid_state (fold_left
+        (fun '(s_acc, obs_acc) e =>
+          let '(s', new_obs) := dual_interp_instr s_acc e in
+          (s', obs_acc ++ new_obs))
+        instrs (s_init, obs_init)).1.
+    Proof.
+      induction instrs as [| e rest IH]; intros s_init obs_init Hvalid.
+      - simpl. exact Hvalid.
+      - simpl. destruct (dual_interp_instr s_init e) as [s' new_obs] eqn:Hstep.
+        apply IH.
+        assert (Hv := dual_interp_preserves_valid s_init e).
+        rewrite Hstep in Hv. simpl in Hv. exact Hv.
+    Qed.
+
+    Lemma run_preserves_valid : forall (s : state) (prog : list instr) (steps : nat),
+      valid_state s -> valid_state (run s prog steps).1.
+    Proof. intros s prog steps H. unfold run. apply fold_left_run_valid. exact H. Qed.
+
     
 
+    (* HW counting *)
 
-  
+    Lemma fold_left_plus : forall (rest : list bool) (acc : nat),
+      fold_left (fun (acc : nat) (b : bool) => if b then acc + 1 else acc) rest acc
+      = fold_left (fun (acc : nat) (b : bool) => if b then acc + 1 else acc) rest 0 + acc.
+    Proof.
+      induction rest. simpl. reflexivity.
+      simpl. intros. destruct a; auto. rewrite IHrest. rewrite IHrest with (acc := 1). lia.
+    Qed.
+
+    Lemma num_true_complement : forall (bools : list bool),
+      num_true bools + num_true (map negb bools) = length bools.
+    Proof.
+      induction bools as [| b rest IH]; simpl.
+      - reflexivity.
+      - unfold num_true in *. simpl filter.
+        destruct b; simpl. rewrite fold_left_plus. lia. rewrite fold_left_plus with (acc := 1). lia.
+    Qed.
+
+    (* Helpers for bv_to_bits_not *)
+    Create HintDb List.
+    Hint Rewrite length_map : List.
+    Hint Rewrite @length_bv_to_bits : List.
+
+    Lemma Some_ne_None' : forall A (opt : option A) a,
+      opt = Some a -> opt <> None.
+    Proof.
+      destruct opt; auto.
+    Qed.
+
+    (* nth_error and stdpp's !! coincide; idx avoids clash with section variable n *)
+    Lemma nth_error_lookup : forall A (xs : list A) (idx : nat) (d : A),
+      nth_error xs idx = xs !! idx.
+    Proof.
+      intros.
+      destruct (list_basics.list.nth_lookup_or_length xs idx d).
+      { rewrite e.
+        apply nth_error_nth'.
+        eapply list_basics.list.lookup_lt_Some; eauto. }
+      { destruct (nth_error _ _) eqn:?.
+        { rewrite <- nth_error_None in l. congruence. }
+        { symmetry. rewrite list_basics.list.lookup_ge_None. auto. } }
+    Qed.
+
+    Lemma bv_to_bits_not : forall (a : bv n),
+      bv_to_bits (bv_not a) = map negb (bv_to_bits a).
+    Proof.
+      intros.
+      apply nth_error_ext.
+      intros. repeat rewrite nth_error_lookup by (try exact false).
+      setoid_rewrite list_monad.list.list_lookup_fmap.
+      destruct (decide (n0 < N.to_nat n)).
+      { repeat match goal with
+        | |- context[?x !! ?y] => destruct (x !! y) eqn:?
+        | H: _ !! _ = None |- _ => rewrite list_basics.list.lookup_ge_None in H
+        | |- Some _ = Some _ => f_equal
+        | |- _ => autorewrite with List in *; auto; try lia; simpl in *
+        end.
+        rewrite bv_to_bits_lookup_Some in *.
+        destruct_and !. subst.
+        rewrite bv_not_unsigned.
+        setoid_rewrite <- Z.lnot_spec; [ | lia].
+        rewrite bv_wrap_spec_low; auto.
+        lia. }
+      { repeat rewrite list_basics.list.lookup_ge_None_2
+          by (autorewrite with List; lia); done. }
+    Qed.
+
+    Lemma hw_complement : forall (a : bv n),
+      HW a + HW (bv_not a) = N.to_nat n.
+    Proof.
+      intro a. unfold HW. rewrite bv_to_bits_not. rewrite num_true_complement.
+      apply length_bv_to_bits.
+    Qed.
+
+    (* General accumulator lemma for HW sums — same pattern as fold_left_plus.
+       NB: parameter named [l] not [env] to avoid the state field projector. *)
+    Lemma num_1s_in_list_fold_plus : forall (l : list (bv n)) (k : nat),
+      fold_left (fun (acc : nat) (pv : bv n) => acc + HW pv) l k =
+      fold_left (fun (acc : nat) (pv : bv n) => acc + HW pv) l 0 + k.
+    Proof.
+      induction l as [| x rest IH]; simpl; intros k.
+      - lia.
+      - rewrite IH. rewrite IH with (k := HW x). lia.
+    Qed.
+
+    Lemma fold_left_plus_HW : forall (l : list (bv n)) (acc : nat) (a : bv n),
+      fold_left (fun (acc : nat) (pv : bv n) => acc + HW pv) l (acc + (HW a))
+      = fold_left (fun (acc : nat) (pv : bv n) => acc + HW pv) l (HW a) + acc.
+    Proof.
+      intros.
+      rewrite num_1s_in_list_fold_plus.
+      rewrite num_1s_in_list_fold_plus with (k := HW a).
+      lia.
+    Qed.
+
+    Lemma valid_state_num_1s_induct : forall (env0 : Env) (acc : nat),
+      fold_left (λ (acc : nat) (pv : bv n), acc + HW pv) env0 acc +
+      fold_left (λ (acc : nat) (pv : bv n), acc + HW pv) (map bv_not env0) acc =
+      length env0 * N.to_nat n + 2 * acc.
+    Proof.
+      (* induction before intros acc so the IH generalises over acc *)
+      induction env0 as [| a rest IH].
+      - simpl. lia.
+      - simpl. intros acc.
+        (* shift both accumulators to 0 using the general fold-left lemma *)
+        rewrite (num_1s_in_list_fold_plus rest).
+        rewrite (num_1s_in_list_fold_plus (map bv_not rest)).
+        (* IH at acc=0: fold rest 0 + fold (map bv_not rest) 0 = length rest * n *)
+        pose proof (IH 0) as IH0.
+        (* hw_complement: HW a + HW (bv_not a) = n *)
+        pose proof (hw_complement a) as Hc.
+        (* simpl already expanded S (length rest) * n and 2 * acc; lia closes *)
+        lia.
+    Qed.
+
+    Lemma valid_state_num_1s : forall (s : state),
+      valid_state s ->
+      num_1s_in_state s = length s.(env) * N.to_nat n.
+    Proof.
+      intros. unfold valid_state in *. unfold num_1s_in_state, num_1s_in_list. rewrite H.
+      destruct s. simpl in *. rewrite valid_state_num_1s_induct. lia.
+    Qed.
+
+
+
+    (* Main security theorem *)
+
+    Lemma all_secure : forall (prog : list instr) (init_s : state),
+      valid_state init_s -> secure prog init_s.
+    Proof.
+      unfold secure. intros prog init_s Hvalid.
+      exists (length init_s.(env) * N.to_nat n). intros steps.
+      rewrite (valid_state_num_1s _ (run_preserves_valid init_s prog steps Hvalid)).
+      rewrite run_preserves_length. reflexivity.
+    Qed.
+
+    
+
+    (* secret register vs public *)
+
+    Inductive RegClass := | SecretReg | PublicReg.
+
+    (* In the ladder X1 and A24 are public inputs, everything else is secret *)
+    Definition ladder_classify (r : var) : RegClass :=
+      match r with
+      | 0 => PublicReg   (* rX1 - base point, known to attacker *)
+      | 5 => PublicReg   (* rA24 — curve constant, public *)
+      | _ => SecretReg
+      end.
+
+    (* sum HW only over a given list of register indices *)
+    Definition num_1s_regs (env : Env) (regs : list var) : nat :=
+      fold_left (fun acc r => acc + HW (read_register env r)) regs 0.
+
+    (* secret register indices for the ladder program *)
+    Definition ladder_secret_regs : list var :=
+      [ rX2; rZ2; rX3; rZ3
+      ; rU; rV; rW; rT
+      ; rU2; rV2; rUT; rVW
+      ; rSp; rSm; rX3'; rSm2; rZ3'
+      ; rX2'; rD; rAD; rT2; rZ2' ].
+
+    (* total HW of secret registers across both sides of dual circuit *)
+    Definition num_1s_secret_state (s : state) (regs : list var) : nat :=
+      num_1s_regs s.(env) regs + num_1s_regs s.(denv) regs.
+
+    (* security focused on secret registers only *)
+    Definition secure_secret (prog : list instr) (s : state) (regs : list var) :=
+      exists c, forall steps,
+        num_1s_secret_state (run s prog steps).1 regs = c.
+
+    (* helper: reading from a complemented env gives the complement *)
+    Lemma read_register_map_not : forall (env : Env) (r : var),
+      r < length env ->
+      read_register (map bv_not env) r = bv_not (read_register env r).
+    Proof.
+      intros env r Hr. unfold read_register.
+      unfold default_var. rewrite <- map_nth with (f := bv_not). apply nth_indep. rewrite length_map. auto.
+    Qed.
+
+    (* fold_left accumulator lemma for num_1s_regs — same pattern as fold_left_plus.
+       NB: parameter named [e] not [env] to avoid shadowing the state field projector. *)
+    Lemma num_1s_regs_fold_plus : forall (e : Env) (regs : list var) (acc : nat),
+      fold_left (fun (acc : nat) (r : var) => acc + HW (read_register e r)) regs acc =
+      fold_left (fun (acc : nat) (r : var) => acc + HW (read_register e r)) regs 0 + acc.
+    Proof.
+      induction regs as [| r rest IH]; simpl; intros acc.
+      - lia.
+      - rewrite IH. rewrite IH with (acc := HW (read_register e r)). lia.
+    Qed.
+
+    (* peeling the head off num_1s_regs *)
+    Lemma num_1s_regs_cons : forall (e : Env) (r : var) (regs : list var),
+      num_1s_regs e (r :: regs) = HW (read_register e r) + num_1s_regs e regs.
+    Proof.
+      intros e r regs. unfold num_1s_regs. simpl.
+      rewrite num_1s_regs_fold_plus. lia.
+    Qed.
+
+    (* HW of secret registers is constant under valid_state *)
+    Lemma valid_state_num_1s_regs : forall (s : state) (regs : list var),
+      valid_state s ->
+      (forall r, In r regs -> r < length s.(env)) ->
+      num_1s_secret_state s regs = length regs * N.to_nat n.
+    Proof.
+      intros s regs Hvalid.
+      (* introduce Hbounds AFTER induction so the IH generalises it for the tail *)
+      induction regs as [| r rest IH]; intros Hbounds.
+      - (* nil: both sides 0 *)
+        unfold num_1s_secret_state, num_1s_regs. simpl. lia.
+      - unfold num_1s_secret_state.
+        rewrite !num_1s_regs_cons.
+        (* head register: HW(env[r]) + HW(denv[r]) = n *)
+        assert (Hstep : HW (read_register s.(env) r) + HW (read_register s.(denv) r) = N.to_nat n).
+        { rewrite Hvalid.
+          rewrite read_register_map_not.
+          - apply hw_complement.
+          - apply Hbounds. left. reflexivity. }
+        (* tail: IH applies with bounds restricted to rest *)
+        assert (IHapp : num_1s_secret_state s rest = length rest * N.to_nat n).
+        { apply IH. intros r' Hr'. apply Hbounds. right. exact Hr'. }
+        unfold num_1s_secret_state in IHapp.
+        simpl length. lia.
+    Qed.
+
+    (* HW of secret registers is constant throughout execution *)
+    Lemma all_secure_secret : forall (prog : list instr) (init_s : state),
+      valid_state init_s ->
+      (forall r, In r ladder_secret_regs -> r < length init_s.(env)) ->
+      secure_secret prog init_s ladder_secret_regs.
+    Proof.
+      unfold secure_secret. intros prog init_s Hvalid Hbounds.
+      exists (length ladder_secret_regs * N.to_nat n).
+      intros steps.
+      apply valid_state_num_1s_regs.
+      - apply run_preserves_valid. exact Hvalid.
+      - (* run preserves register bounds - needs a lemma? *)
+        admit.
+    Admitted.
+
+    (* Compact register allocation *)
+
+    Notation cX1  := 0  (only parsing).   (* public: base point x-coord     *)
+    Notation cX2  := 1  (only parsing).   (* secret                          *)
+    Notation cZ2  := 2  (only parsing).   (* secret                          *)
+    Notation cX3  := 3  (only parsing).   (* secret                          *)
+    Notation cZ3  := 4  (only parsing).   (* secret                          *)
+    Notation cA24 := 5  (only parsing).   (* public: curve constant          *)
+    Notation cT0  := 6  (only parsing).   (* temp, reused across the step   *)
+    Notation cT1  := 7  (only parsing).   (* temp                             *)
+    Notation cT2  := 8  (only parsing).   (* temp                            *)
+    Notation cT3  := 9  (only parsing).   (* temp                            *)
+    Notation cT4  := 10 (only parsing).   (* temp                            *)
+    Notation cT5  := 11 (only parsing).   (* temp                            *)
+
+    Definition compact_program : list instr :=
+      [ IAdd cT0  cX2  cZ2    (* T0 = X2+Z2        = U                       *)
+      ; ISub cT1  cX2  cZ2    (* T1 = X2−Z2        = V                       *)
+      ; IAdd cT2  cX3  cZ3    (* T2 = X3+Z3        = W                       *)
+      ; ISub cT3  cX3  cZ3    (* T3 = X3−Z3        = T                       *)
+      ; IMul cT4  cT0  cT0    (* T4 = U·U          = U²                      *)
+      ; IMul cT5  cT1  cT1    (* T5 = V·V          = V²   [peak: 8 live]     *)
+      ; IMul cT0  cT0  cT3    (* T0 = U·T          = UT   [T3 dead]          *)
+      ; IMul cT3  cT1  cT2    (* T3 = V·W          = VW   [T1,T2 dead]       *)
+      ; IAdd cT1  cT0  cT3    (* T1 = UT+VW        = Sp                      *)
+      ; ISub cT2  cT0  cT3    (* T2 = UT−VW        = Sm   [T0,T3 dead]       *)
+      ; IMul cT1  cT1  cT1    (* T1 = Sp·Sp        = X3'                     *)
+      ; IMul cT0  cT2  cT2    (* T0 = Sm·Sm        = Sm²  [T2 dead]          *)
+      ; IMul cT2  cT0  cX1    (* T2 = Sm²·X1       = Z3'  [T0,X1 dead]       *)
+      ; IMul cT0  cT4  cT5    (* T0 = U²·V²        = X2'                     *)
+      ; ISub cT3  cT4  cT5    (* T3 = U²−V²        = D    [T4 dead]          *)
+      ; IMul cT4  cA24 cT3    (* T4 = A24·D        = AD   [A24 dead]         *)
+      ; IAdd cT5  cT5  cT4    (* T5 = V²+AD        = T2'  [T5,T4 dead]       *)
+      ; IMul cT3  cT3  cT5    (* T3 = D·T2'        = Z2'  [T3,T5 dead]       *)
+      ].
+      (* Final: cT0=X2', cT1=X3', cT2=Z3', cT3=Z2'  (4 output regs)         *)
+
+    (* Generalised public/secret classification
+       declare a list of public registers --> derive the classify function from it *)
+
+    Definition classify_by_list (pub : list var) (r : var) : RegClass :=
+      if decide (r ∈ pub) then PublicReg else SecretReg.
+
+    (* Retrofit the original program with the general classifier *)
+    Definition ladder_public_regs : list var := [rX1; rA24].  (* 0 and 5     *)
+    Definition ladder_classify' : var -> RegClass :=
+      classify_by_list ladder_public_regs.
+
+    (* Compact program: same two public inputs, same physical register slots  *)
+    Definition compact_public_regs : list var := [cX1; cA24].  (* also 0,5   *)
+    Definition compact_classify : var -> RegClass :=
+      classify_by_list compact_public_regs.
+
+    (* Secret registers for the compact program (everything except public)    *)
+    Definition compact_secret_regs : list var :=
+      [cX2; cZ2; cX3; cZ3; cT0; cT1; cT2; cT3; cT4; cT5].
+
+    (* HW of secret registers in compact program is constant
+       same proof structure as all_secure_secret?  *)
+    Lemma compact_all_secure_secret : forall (init_s : state),
+      valid_state init_s ->
+      (forall r, In r compact_secret_regs -> r < length init_s.(env)) ->
+      secure_secret compact_program init_s compact_secret_regs.
+    Proof.
+      unfold secure_secret. intros init_s Hvalid Hbounds.
+      exists (length compact_secret_regs * N.to_nat n).
+      intros steps.
+      apply valid_state_num_1s_regs.
+      - apply run_preserves_valid. exact Hvalid.
+      - intros r Hr.
+        rewrite run_preserves_length. apply Hbounds. exact Hr.
+    Admitted.  (* valid_state_num_1s_regs *)
+
+    (* 1. set of public registers --> public are not duplicated *)
+        (* ISA contract? write another update function where only have shadow regs for secret *)
+
+    (* run function on env --> list of obs --> functional correctness hold across run on env and on goal circuit *)
+      (* definition of functional correctness - how to state *)
+    (* observation of circuit & dual same at every  *)
+
+    (* add memory? *)
+      (* define machine: consists of registers & a memory --> 1. InstrMem: list of instructions (alt: store as bv --> translate to instr
+         2. DataMem: store secret & public data
+        --> implement a simple processor: program counter (also public), fetch --> memory respond in 1 cycle with instruction -->
+         decode execute in single cycle *)
+    (* hardware-software contract? *)
+    (* language?  *)
+    (* duplicate dynamically? some registers are 0 until you allocate a pair *)
+  End DualCircuit.
+
+  (* normal probability theory *)
+  (* standard probability notation? *)
+  (* probability > normal draws -->  *)
+  (* justify from first principle? *)
+    (* probability defined - in information theory library? *)
+
+  (* end goal: number of 1's per cycle *)
+  (* cryptographic accelerator? *)
+
+  (* whether the number of 1's is the right metric of measuring power? *)
 
 End HammingWeight.
+
+(* Pipeline stages as an enum — mutually exclusive, exactly one active per cycle *)
+Inductive PipelineStage :=
+  | Fetch
+  | Execute
+  | WriteBack.
+
+Module StateMachine.
+Section StateMachine.
+  Variable n : N.
+
+  (* secret_map.(j) names which Regs slot is duplicated into DRegs slot j.
+     e.g. secret_map.[0] = Fin 3 means DRegs[0] mirrors Regs[3].          *)
+  Variable secret_map : Vector.t (Fin.t 32) 16.
+
+  Record state := mkState {
+    pc        : bv n;
+    Regs      : Vector.t (bv n) 32;      (* all 32 general-purpose registers   *)
+    DRegs     : Vector.t (bv n) 16;      (* dual of the 16 secret registers    *)
+    InstrMem  : list instr;              (* program — public                   *)
+    DataMem   : nat -> bv n;             (* data heap                          *)
+    Stage     : PipelineStage;           (* current pipeline stage             *)
+    (* instruction memory bus — public: carries opcodes, no duplication needed *)
+    toiMem    : bool * bv n;             (* (valid, fetch addr)                *)
+    fromiMem  : bool * bv n;             (* (valid, fetched instr)             *)
+    (* data memory bus — may carry secret values, so dualized                  *)
+    todMem    : bool * bv n * bv n;      (* (valid, addr, data)   write bus    *)
+    dtodMem   : bool * bv n * bv n;      (* dual write bus                     *)
+    fromdMem  : bool * bv n;             (* (valid, loaded data)  read bus     *)
+    dfromdMem : bool * bv n;             (* dual read bus                      *)
+  }.
+
+  (* Invariant: every dual register is the bitwise complement of its secret original.
+     DRegs[j] = bv_not (Regs[secret_map[j]])  for all j : Fin.t 16            *)
+  Definition valid_state (s : state) : Prop :=
+    forall j : Fin.t 16,
+      Vector.nth s.(DRegs) j =
+      bv_not (Vector.nth s.(Regs) (Vector.nth secret_map j)).
+
+  (* Stage handlers — admitted until we flesh out the ISA semantics *)
+  Definition fetch     : state -> state. Admitted.
+  Definition execute   : state -> state. Admitted.
+  Definition writeback : state -> state. Admitted.
+
+  (* One clock tick: dispatch on the current pipeline stage *)
+  Definition tick (s : state) : state :=
+    match s.(Stage) with
+    | Fetch     => fetch s
+    | Execute   => execute s
+    | WriteBack => writeback s
+    end.
+
+  (* Memory-side ticks — admitted until bus protocol is defined *)
+  Definition tick_dMem : state -> state. Admitted.
+  Definition tick_iMem : state -> state. Admitted.
+
+  (* ── Security theorems ───────────────────────────────────────────────────── *)
+
+  (* valid_state is preserved by each tick *)
+  Lemma tick_preserves_valid : forall (s : state),
+    valid_state s -> valid_state (tick s).
+  Proof.
+  Admitted.
+
+  (* total HW of secret registers + their duals is constant per cycle *)
+  (* (same dual-circuit argument as all_secure_secret, now for a full processor) *)
+
+End StateMachine.
+End StateMachine.
